link.v
@@ -1,5 +1,6 @@
 (** Verification of Give-up template algorithm *)
 
+Require Import lock.
 From iris.algebra Require Import excl auth gmap agree gset frac.
 From iris.heap_lang Require Export lifting notation locations lang.
 From iris.base_logic.lib Require Export invariants.
@@ -67,20 +68,6 @@ Section Link_Template.
 
   Parameter findNext : val.
   Parameter decisiveOp : (dOp → val).
-  Parameter lockLoc : Node → loc.
-  Parameter getLockLoc : val.
-
-  Definition lockNode : val :=
-    rec: "lockN" "x" :=
-      let: "l" := getLockLoc "x" in
-      if: CAS "l" #false #true
-      then #()
-      else "lockN" "x".
-
-  Definition unlockNode : val :=
-    λ: "x",
-    let: "l" := getLockLoc "x" in
-    "l" <- #false.
 
   Definition traverse : val :=
     rec: "tr" "n" "k" :=
@@ -129,11 +116,6 @@ Section Link_Template.
   (** Helper functions specs *)
   (* These are proved for each implementation in GRASShopper *)
 
-  Parameter getLockLoc_spec : ∀ (n: Node),
-      ⊢ ({{{ True }}}
-           getLockLoc #n
-         {{{ (l:loc), RET #l; ⌜lockLoc n = l⌝ }}})%I.
-
   (* The following functions are proved for each implementation in GRASShopper
    * (see b-link.spl and hashtbl-link.spl *)
 
@@ -172,47 +154,6 @@ Section Link_Template.
 
   Definition is_CSS γ γ_fp γ_k γ_inr γ_fi root C :=
     (∃ I, (CSS γ γ_fp γ_k γ_inr γ_fi root I C))%I.
-
-  (** Lock module proofs *)
-
-  Lemma lockNode_spec (n: Node):
-    ⊢ <<< ∀ (b: bool), (lockLoc n) ↦ #b >>>
-        lockNode #n    @ ⊤
-      <<< (lockLoc n) ↦ #true ∗ ⌜b = false⌝, RET #() >>>.
-  Proof.
-    iIntros (Φ) "AU". iLöb as "IH".
-    wp_lam. wp_bind(getLockLoc _)%E.
-    wp_apply getLockLoc_spec; first done.
-    iIntros (l) "#Hl". wp_let. wp_bind (CmpXchg _ _ _)%E.
-    iMod "AU" as (b) "[Hb HAU]". iDestruct "Hl" as %Hl.
-    iEval (rewrite Hl) in "Hb". destruct b.
-    - wp_cmpxchg_fail. iDestruct "HAU" as "[HAU _]".
-      iEval (rewrite Hl) in "HAU".
-      iMod ("HAU" with "Hb") as "H".
-      iModIntro. wp_pures. iApply "IH".
-      iEval (rewrite <-Hl) in "H". done.
-    - wp_cmpxchg_suc. iDestruct "HAU" as "[_ HAU]".
-      iEval (rewrite Hl) in "HAU".
-      iMod ("HAU" with "[Hb]") as "HΦ". iFrame; done.
-      iModIntro. wp_pures. done.
-  Qed.
-
-  Lemma unlockNode_spec (n: Node) :
-    ⊢ <<< lockLoc n ↦ #true >>>
-        unlockNode #n    @ ⊤
-      <<< lockLoc n ↦ #false, RET #() >>>.
-  Proof.
-    iIntros (Φ) "AU". wp_lam. wp_bind(getLockLoc _)%E.
-    wp_apply getLockLoc_spec; first done.
-    iIntros (l) "#Hl". wp_let.
-    iMod "AU" as "[Hy [_ Hclose]]".
-    iDestruct "Hl" as %Hl.
-    iEval (rewrite Hl) in "Hy".
-    wp_store. iEval (rewrite Hl) in "Hclose".
-    iMod ("Hclose" with "Hy") as "HΦ".
-    iModIntro. done.
-  Qed.
-
 
   (** Proofs of traverse and CSSOp *)
 
